Cherry picking clone methods for Bytes

CoqOfRust/revm/links/dependencies.v
@@ -1,12 +1,33 @@
 Require Import CoqOfRust.CoqOfRust.
 Require Import CoqOfRust.links.M.
+Require core.links.clone.
+
+Module ruint.
+  Module Uint.
+    Parameter t : Usize.t -> Usize.t -> Set.
+
+    Parameter to_value : forall {BITS LIMBS : Usize.t}, t BITS LIMBS -> Value.t.
+
+    Global Instance IsLink : forall {BITS LIMBS : Usize.t}, Link (t BITS LIMBS) := {
+      Φ := Ty.apply (Ty.path "ruint::Uint") [ φ BITS; φ LIMBS ] [];
+      φ := to_value;
+    }.
+
+    Definition of_ty (BITS' LIMBS' : Value.t) (BITS LIMBS : Usize.t) :
+      BITS' = φ BITS ->
+      LIMBS' = φ LIMBS ->
+      OfTy.t (Ty.apply (Ty.path "ruint::Uint") [ BITS' ; LIMBS' ] []).
+    Proof. intros. eapply OfTy.Make with (A := t BITS LIMBS). now subst. Defined.
+    Smpl Add eapply of_ty : of_ty.
+  End Uint.
+End ruint.
 
 Module alloy_primitives.
   Module bits.
     Module links.
       Module address.
         Module Address.
-          Parameter t: Set.
+          Parameter t : Set.
 
           Parameter to_value : t -> Value.t.
 
@@ -27,10 +48,39 @@ Module alloy_primitives.
         Parameter to_value : t -> Value.t.
 
         Global Instance IsLink : Link t := {
-          Φ := Ty.path "bytes::bytes::Bytes";
+          Φ := Ty.path "alloy_primitives::bytes_::Bytes";
           φ := to_value;
         }.
+
+        Definition of_ty : OfTy.t (Ty.path "alloy_primitives::bytes_::Bytes").
+        Proof. eapply OfTy.Make with (A := t); reflexivity. Defined.
+        Smpl Add apply of_ty : of_ty.
       End Bytes.
+      
+      Module Impl_Clone_for_Bytes.
+        Definition Self : Ty.t := Ty.path "alloy_primitives::bytes_::Bytes".
+
+        Parameter clone : PolymorphicFunction.t.
+
+        Axiom Implements :
+          M.IsTraitInstance
+            "core::clone::Clone"
+            (* Trait polymorphic consts *) []
+            (* Trait polymorphic types *) []
+            Self
+            (* Instance *) [ ("clone", InstanceField.Method clone) ].
+
+        Definition run_clone : clone.Clone.Run_clone Bytes.t.
+        Admitted.
+      
+        Definition run : clone.Clone.Run Bytes.t.
+        Proof.
+          constructor.
+          { (* clone *)
+            exact run_clone.
+          }
+        Defined.
+      End Impl_Clone_for_Bytes.
     End bytes_.
   End links.
 End alloy_primitives.
@@ -45,7 +95,6 @@ Module Address.
     φ := to_value;
   }.
 End Address.
-
 Module FixedBytes.
   Parameter t : Set.
 
